examples/low-level/crypto/Crypto.AEAD.Wrappers.CMA.fst
@@ -1,0 +1,266 @@
+module Crypto.AEAD.Wrappers.CMA
+open FStar.UInt32
+open FStar.Ghost
+open Buffer.Utils
+open FStar.Monotonic.RRef
+
+open Crypto.Indexing
+open Crypto.Symmetric.Bytes
+open Crypto.Plain
+open Flag
+
+open Crypto.Symmetric.PRF
+open Crypto.AEAD.Invariant
+open Crypto.AEAD.Encoding
+
+module Cipher = Crypto.Symmetric.Cipher
+module PRF = Crypto.Symmetric.PRF
+module Plain = Crypto.Plain
+module Invariant = Crypto.AEAD.Invariant
+module HH = FStar.HyperHeap
+module HS = FStar.HyperStack
+module CMA = Crypto.Symmetric.UF1CMA
+module SeqProperties = FStar.SeqProperties
+module MAC = Crypto.Symmetric.MAC
+
+(*** UF1CMA.mac ***)
+#reset-options "--z3rlimit 40 --initial_fuel 0 --max_fuel 0 --initial_ifuel 0 --max_ifuel 0"
+let mac_ensures (i:CMA.id) (st:CMA.state i) (acc:CMA.accBuffer i) (tag:MAC.tagB)
+		(h0:mem) (h1:mem) = 
+    let open FStar.Buffer in
+    let open Crypto.Symmetric.Bytes in
+    let open Crypto.Symmetric.Poly1305 in
+    let open Crypto.Symmetric.UF1CMA in
+    Buffer.live h0 st.s /\ 
+    MAC.live h0 st.r /\ 
+    Buffer.live h1 tag /\
+    CMA.acc_inv st acc h0 /\ (
+    if mac_log then
+      HS.modifies (Set.as_set [st.region; Buffer.frameOf tag]) h0 h1 /\
+      Buffer.modifies_buf_1 (Buffer.frameOf tag) tag h0 h1 /\
+      HS.modifies_ref st.region !{HS.as_ref (as_hsref (ilog st.log))} h0 h1 /\
+      m_contains (ilog st.log) h1 /\ (
+      let log = FStar.HyperStack.sel h1 (alog acc) in
+      let a = MAC.sel_elem h1 (abuf acc) in
+      let r = MAC.sel_elem h1 st.r in
+      let s = Buffer.as_seq h1 st.s in
+      let t = MAC.mac log r s in
+      sel_word h1 tag === t /\
+      m_sel h1 (ilog st.log) == Some(log,t))
+    else Buffer.modifies_1 tag h0 h1)
+
+let mac_wrapper (#i:CMA.id) (st:CMA.state i) (acc:CMA.accBuffer i) (tag:MAC.tagB)
+  : ST unit
+  (requires (fun h0 ->
+    let open Crypto.Symmetric.UF1CMA in
+    Buffer.live h0 tag /\ 
+    Buffer.live h0 st.s /\
+    Buffer.disjoint_2 (MAC.as_buffer (abuf acc)) st.s tag /\
+    Buffer.disjoint (MAC.as_buffer st.r) tag /\
+    Buffer.disjoint st.s tag /\ 
+    acc_inv st acc h0 /\
+    (mac_log ==> m_contains (ilog st.log) h0) /\
+    (mac_log /\ authId i ==> m_sel h0 (ilog st.log) == None)))
+  (ensures (fun h0 _ h1 -> mac_ensures i st acc tag h0 h1))
+  = let open Crypto.Symmetric.UF1CMA in
+    let h0 = get () in
+    CMA.mac #i st acc tag;
+    let h1 = get () in 
+    if mac_log then begin
+      (* Need to update UF1CMA to prove this (problem with the mods clause not working fully) *)
+      assume (HS.modifies_ref st.region !{HS.as_ref (as_hsref (ilog st.log))} h0 h1) //NS: this goes away when UF1CMA is done
+    end
+
+(*** UF1CMA.verify ***)
+
+(*+ The main work of wrapping UF1CMA.verify is to 
+    establish that when called with the AEAD.Invariant.inv, 
+    if verify returns true for a particular encoded AD+cipher, 
+    then in the ideal case, we can also return the plain text
+    expected for the result of decryption **)
+    
+(*+ found_entry: 
+      the entry in the aead table corresponding to nonce n
+      contains the expected aad, plain and cipher text
+ **)
+let found_entry (#i:id) (n:Cipher.iv (Cipher.algi i)) (st:aead_state i Reader)
+		(#aadlen:aadlen) (aad:lbuffer (v aadlen)) 
+	        (#plainlen:txtlen_32 {safelen i (v plainlen) (PRF.ctr_0 i +^ 1ul)})
+		(cipher_tagged:lbuffer (v plainlen + v MAC.taglen))
+		(q:maybe_plain i (v plainlen))
+		(h:mem) =
+    (Buffer.live h cipher_tagged /\
+     Buffer.live h aad /\
+     safeId i) ==> 		
+    (let entries = HS.sel h st.log in 		
+     match find_aead_entry n entries with
+     | None -> False
+     | Some (AEADEntry nonce ad l p c) ->
+         nonce == n /\
+	 ad == Buffer.as_seq h aad /\
+	 l  == v plainlen /\
+	 c  == Buffer.as_seq h cipher_tagged /\ 
+	 p  == as_plain q )
+
+(*+ verify_liveness: 
+	liveness pre-condition for calling UF1CMA.verify **)
+let verify_liveness (#i:CMA.id) (st:CMA.state i) (tag:lbuffer 16) (h:mem) =
+    Buffer.live h (CMA.(st.s)) /\
+    Buffer.live h (CMA.(MAC.as_buffer st.r)) /\
+    Buffer.live h tag
+
+(*+ verify_ok: 
+	post-condition of verify
+	
+	Notably, if verify returnes true, then the mac log contains 
+	the expected tag
+  **)	
+let verify_ok (#i:CMA.id) (st:CMA.state i) (acc:CMA.accBuffer i) (tag:lbuffer 16) 
+		     (h:mem{verify_liveness st tag h}) (b:bool)  = 
+    let open Crypto.Symmetric.UF1CMA in
+    if mac_log then 
+      let log = FStar.HyperStack.sel h (alog acc) in
+      let r = MAC.sel_elem h st.r in
+      let s = Buffer.as_seq h st.s in
+      let m = MAC.mac log r s in
+      let verified = Seq.eq m (MAC.sel_word h tag) in
+      if authId i then
+      	match m_sel h (ilog st.log) with
+      	| Some(l',m') ->
+      	  let correct = m = m' && Seq.eq log l' in
+      	  b == (verified && correct)
+      	| None -> b==false
+      else b==verified
+    else True
+
+(*+ is_mac_for_iv:
+	ak being indexed for (i, n)
+
+	really corresponds to the ak being the stored mac in the prf table for n
+ **)
+let is_mac_for_iv (#i:id) (#n:Cipher.iv (alg i)) (st:aead_state i Reader{safeId i}) (ak:CMA.state (i, n)) (h:mem) = 
+  let x0 = {iv=n; ctr=ctr_0 i} in 
+  match find_mac (HS.sel h (itable i st.prf)) x0 with 
+  | Some mac -> ak == mac
+  | _ -> False
+
+(*+ accumulate_encoded:
+      the post-condition of accumulate ... 
+      just a wrapper around encode_both
+ **)      
+let accumulate_encoded (#i:CMA.id)
+ 		       (#aadlen:aadlen) (aad:lbuffer (v aadlen))
+		       (#plainlen:txtlen_32) (cipher:lbuffer (v plainlen))
+		       (a:CMA.accBuffer i) (h:mem{mac_log}) =
+    Buffer.live h aad /\			 
+    Buffer.live h cipher /\			     
+    h `HS.contains` (CMA.alog a) /\
+    HS.sel h (CMA.alog a) ==
+    encode_both (fst i) aadlen (Buffer.as_seq h aad) plainlen (Buffer.as_seq h cipher)
+
+(*+ entry_exists_if_verify_ok:
+	A key lemma from the invariant and verify succeeding
+
+        It establishes that if verify succeeds on an encoded ad+cipher
+	then there is a corresponding entry in the aead_table with the
+	ad, cipher and some plaintext 
+ **)	
+val entry_exists_if_verify_ok : #i:id -> #n:Cipher.iv (alg i) -> (st:aead_state i Reader) ->
+ 			        #aadlen:aadlen -> aad:lbuffer (v aadlen) ->
+			        #plainlen:txtlen_32 {safelen i (v plainlen) (otp_offset i)} ->
+			       (plain:Plain.plainBuffer i (v plainlen)) ->
+			       (cipher_tagged:lbuffer (v plainlen + v MAC.taglen)) ->
+			       (ak:CMA.state (i,n)) ->
+			       (acc:CMA.accBuffer (i, n)) ->
+			       (tag:lbuffer 16{tag == Buffer.sub cipher_tagged plainlen MAC.taglen}) ->
+			       (h:mem{enc_dec_liveness st aad plain cipher_tagged h /\
+				      verify_liveness ak tag h /\ 
+				      safeId i}) ->
+   Lemma (requires (inv st h /\
+		    CMA.acc_inv ak acc h /\
+		    accumulate_encoded aad #plainlen (Buffer.sub cipher_tagged 0ul plainlen) acc h /\
+		    verify_ok ak acc tag h true /\
+		    is_mac_for_iv st ak h))
+         (ensures (match find_aead_entry n (HS.sel h st.log) with
+		   | None -> False
+		   | Some (AEADEntry _ _ l p _) ->
+		     l == v plainlen /\
+		     found_entry n st aad cipher_tagged p h))
+#reset-options "--initial_ifuel 0 --max_ifuel 0 --initial_fuel 0 --max_fuel 0 --z3rlimit 400"
+let entry_exists_if_verify_ok #i #n st #aadlen aad #plainlen plain cipher_tagged_b ak acc tag_b h =
+    let aead_entries = HS.sel h st.log in
+    let prf_table = HS.sel h (PRF.itable i st.prf) in
+    let x0 = {iv = n; ctr=ctr_0 i} in
+    let cipher_tagged = Buffer.as_seq h cipher_tagged_b in
+    let cipher, _ = SeqProperties.split cipher_tagged (v plainlen) in
+    let tag = Buffer.as_seq h tag_b in
+    let aead_entry = find_refined_aead_entry n aead_entries prf_table h in 
+    let Some ak' = PRF.find_mac prf_table x0 in
+    assert (ak == ak');
+    let AEADEntry nonce aad' plainlen' p' cipher_tagged' = aead_entry in
+    let cipher', _ = SeqProperties.split cipher_tagged' plainlen' in
+    let mac_log = CMA.ilog (CMA.State?.log ak) in
+    match m_sel h mac_log with
+    | None           -> ()
+    | Some (msg,tag') -> 
+      lemma_encode_both_inj i aadlen plainlen (u (Seq.length aad')) (u plainlen')
+			     (Buffer.as_seq h aad) cipher aad' cipher';
+      assert (Seq.equal tag tag');
+      assert (Seq.equal cipher cipher');
+      assert (Seq.equal cipher_tagged' (Seq.append cipher' tag'));
+      assert (Seq.equal cipher_tagged (Seq.append cipher tag))
+
+(*+ get_verified_plain: 
+       The main additional work of the UF1CMA.verify wrapper
+
+       In case verify succeeds, we call this function in the ideal
+       case to extract the plain text from the aead table and return
+       it to decrypt, which in turn uses it to state and establish the
+       invariant of counter_dexor
+ **)
+val get_verified_plain : #i:id -> #n:Cipher.iv (alg i) -> st:aead_state i Reader ->
+ 			 #aadlen:aadlen -> (aad:lbuffer (v aadlen)) ->
+			 #plainlen:txtlen_32 {plainlen <> 0ul /\ safelen i (v plainlen) (PRF.ctr_0 i +^ 1ul)} ->
+			 plain:Plain.plainBuffer i (v plainlen) ->
+			 cipher_tagged:lbuffer (v plainlen + v MAC.taglen) ->
+		         ak:CMA.state (i,n) ->
+			 acc:CMA.accBuffer (i, n) ->
+			 verified:bool ->
+      ST (maybe_plain i (v plainlen))
+         (requires (fun h -> 
+		    let tag = Buffer.sub cipher_tagged plainlen MAC.taglen in 
+		    enc_dec_liveness st aad plain cipher_tagged h /\ 
+		    (if safeId i && verified
+		     then verify_liveness ak tag h /\ 
+		  	  is_mac_for_iv st ak h /\
+			  inv st h /\
+			  CMA.acc_inv ak acc h /\
+			  accumulate_encoded aad #plainlen (Buffer.sub cipher_tagged 0ul plainlen) acc h /\
+			  verify_ok ak acc tag h true
+	             else True)))
+         (ensures (fun h0 p h1 -> 
+		    let cipher = Buffer.sub cipher_tagged 0ul plainlen in
+		    let x1 = {iv=n; ctr=otp_offset i} in
+		    h0 == h1 /\
+    		    enc_dec_liveness st aad plain cipher_tagged h1 /\ 
+		    (if verified && safeId i
+		     then prf_contains_all_otp_blocks x1 0 (as_plain p) (Buffer.as_seq h1 cipher) (HS.sel h1 (PRF.itable i st.prf)) /\
+		          found_entry n st aad cipher_tagged p h1
+		     else True)))
+#reset-options "--initial_fuel 0 --max_fuel 0 --initial_ifuel 0 --max_ifuel 0 --z3rlimit 100"
+let get_verified_plain #i #n st #aadlen aad #plainlen plain cipher_tagged ak acc verified = 
+  if safeId i && verified then
+    let h = get () in
+    let tag = Buffer.sub cipher_tagged plainlen MAC.taglen in 
+    entry_exists_if_verify_ok st aad plain cipher_tagged ak acc tag h;
+    let aead_entries = !st.log in 
+    let Some (AEADEntry _nonce _ad _l p _c) = find_aead_entry n aead_entries in
+    let _ : unit = 
+      let prf_table = HS.sel h (PRF.itable i st.prf) in
+      let e = find_refined_aead_entry n aead_entries prf_table h in
+      () in
+    p
+  else if safeId i then 
+     Plain.load plainlen plain
+  else ()
+
